Semantic/ModalCapybara/Syntax.lean
@@ -1,6 +1,7 @@
 import Semantic.ModalCapybara.Syntax.Ty
 import Semantic.ModalCapybara.Syntax.Exp
 import Semantic.ModalCapybara.Syntax.Context
+import Semantic.ModalCapybara.Syntax.Constraint
 
 /-!
 Syntax definitions for CC.
